src/Spec.EDHOC.KeySchedule.fsti
@@ -42,36 +42,51 @@ val construct_info:
   -> context:serializable_bytes
   -> okm_len:okm_len_type
   -> Tot info
-val concat_info_get_length:
-  i:info
-  -> Tot size_nat
+
+inline_for_extraction
+let concat_info_get_length (i:info)
+  : size_nat
+  = (FBytes.repr_bytes i.label)
+    + (length i.context)
+    + (FBytes.repr_bytes i.okm_len)
+
+let lemma_concat_info_get_length_fixed_length
+  (i:info)
+  : Lemma (ensures (
+    concat_info_get_length i = (FBytes.repr_bytes i.label) + (length i.context) + (FBytes.repr_bytes i.okm_len)
+  ))
+  [SMTPat (concat_info_get_length i)]
+  = ()
+  
 val concat_info:
   i:info
   -> Tot (lbytes (concat_info_get_length i))
+
 val construct_info_to_bytes:
   label:info_label
   -> context:serializable_bytes
   -> okm_len:okm_len_type
   -> Tot (lbytes (
-    (FBytes.repr_bytes label) + (length context) + (FBytes.repr_bytes okm_len)
+    concat_info_get_length (construct_info label context okm_len)
   ))
 
-let lemma_construct_info_to_bytes_equiv_concat
-  (label:info_label) (context:serializable_bytes)
-  (okm_len:okm_len_type)
-  : Lemma (ensures (
+val lemma_construct_info_to_bytes_equiv_concat:
+  label:info_label
+  -> context:serializable_bytes
+  -> okm_len:okm_len_type
+  -> Lemma (ensures (
     let info_bytes = construct_info_to_bytes label context okm_len in
     let info_struct = construct_info label context okm_len in
     equal info_bytes (concat_info info_struct)
   ))
   [SMTPat (construct_info_to_bytes label context okm_len)]
-  = ()
 
 // no need to deserialize this info struct
 // as component fields are already-known to the caller.
 val serialize_info_get_length:
   i:info
   -> Tot size_nat
+  
 val serialize_info:
   i:info
   -> Tot (r:lbytes (serialize_info_get_length i))
@@ -87,10 +102,20 @@ val construct_context2:
   -> ead2:option ead_bytes
   -> Tot (context2 #cs)
 
-val concat_context2_get_length:
-  #cs:supported_cipherSuite
-  -> ctx2:context2 #cs
-  -> Tot size_nat
+// val concat_context2_get_length:
+//   #cs:supported_cipherSuite
+//   -> ctx2:context2 #cs
+//   -> Tot size_nat
+
+let concat_context2_get_length
+  (#cs:supported_cipherSuite)
+  (ctx2:context2 #cs)
+  = let ead_len = match ctx2.ead2 with
+                    | None -> 0
+                    | Some ead2 -> length ead2
+                    in 
+  (length ctx2.c_r) + (length ctx2.id_cred_r)
+  + (hash_size cs) + (length ctx2.cred_r) + ead_len
 
 val concat_context2:
   #cs:supported_cipherSuite
@@ -113,17 +138,19 @@ val construct_context2_to_bytes:
     )
   )) 
 
-let lemma_construct_context2_to_bytes_equiv_concat
-  (#cs:supported_cipherSuite) (c_r:c_id_bytes)
-  (id_cred_r:id_cred_i_bytes) (th2:hash_out cs)
-  (cred_r:cred_i_bytes) (ead2:option ead_bytes)
-  : Lemma (ensures (
+val lemma_construct_context2_to_bytes_equiv_concat:
+  #cs:supported_cipherSuite
+  -> c_r:c_id_bytes
+  -> id_cred_r:id_cred_i_bytes
+  -> th2:hash_out cs
+  -> cred_r:cred_i_bytes
+  -> ead2:option ead_bytes
+  -> Lemma (ensures (
     let context2_bytes = construct_context2_to_bytes c_r id_cred_r th2 cred_r ead2 in
     let context2_struct = construct_context2 c_r id_cred_r th2 cred_r ead2 in
     equal context2_bytes (concat_context2 context2_struct)
   ))
   [SMTPat (construct_context2_to_bytes #cs c_r id_cred_r th2 cred_r ead2)]
-  = ()
 
 val serialize_context2_get_length:
   #cs:supported_cipherSuite
@@ -145,10 +172,20 @@ val construct_context3:
   -> ead3:option ead_bytes
   -> Tot (context3 #cs)
 
-val concat_context3_get_length:
-  #cs:supported_cipherSuite
-  -> ctx3:context3 #cs
-  -> Tot size_nat
+// val concat_context3_get_length:
+//   #cs:supported_cipherSuite
+//   -> ctx3:context3 #cs
+//   -> Tot size_nat
+
+let concat_context3_get_length
+  (#cs:supported_cipherSuite)
+  (ctx3:context3 #cs)
+  = let ead_len = match ctx3.ead3 with
+                    | None -> 0
+                    | Some ead3 -> length ead3
+                    in
+  (length ctx3.id_cred_i) + (hash_size cs)
+  + (length ctx3.cred_i) + ead_len
 
 val concat_context3:
   #cs:supported_cipherSuite
@@ -162,23 +199,21 @@ val construct_context3_to_bytes:
   -> cred_i:cred_i_bytes
   -> ead3:option ead_bytes
   -> Tot (lbytes (
-    (length id_cred_i) + (hash_size cs) + (length cred_i) + (
-      match ead3 with
-        | None -> 0
-        | Some v -> length v
-    )
+    concat_context3_get_length (construct_context3 id_cred_i th3 cred_i ead3)
   ))
 
-let lemma_construct_context3_to_bytes_equiv_concat
-  (#cs:supported_cipherSuite) (id_cred_i:id_cred_i_bytes)
-  (th3:hash_out cs) (cred_i:cred_i_bytes) (ead3:option ead_bytes)
-  : Lemma (ensures (
+val lemma_construct_context3_to_bytes_equiv_concat:
+  #cs:supported_cipherSuite
+  -> id_cred_i:id_cred_i_bytes
+  -> th3:hash_out cs
+  -> cred_i:cred_i_bytes
+  -> ead3:option ead_bytes
+  -> Lemma (ensures (
     let context3_bytes = construct_context3_to_bytes id_cred_i th3 cred_i ead3 in
     let context3_struct = construct_context3 id_cred_i th3 cred_i ead3 in
     equal context3_bytes (concat_context3 context3_struct)
   ))
   [SMTPat (construct_context3_to_bytes #cs id_cred_i th3 cred_i ead3)]
-  = ()
 
 val serialize_context3_get_length:
   #cs:supported_cipherSuite
@@ -207,15 +242,16 @@ val extract_prk3e2m:
   -> g_rx:shared_secret cs // key
   -> hash_out cs
 
-let lemma_extract_prk3e2m_equality
-  (#cs:supported_cipherSuite)
-  (salt1:hash_out cs) (salt2:hash_out cs)
-  (ikm1:shared_secret cs) (ikm2:shared_secret cs)
-  : Lemma (requires (
+val lemma_extract_prk3e2m_equality:
+  #cs:supported_cipherSuite
+  -> salt1:hash_out cs
+  -> salt2:hash_out cs
+  -> ikm1:shared_secret cs
+  -> ikm2:shared_secret cs
+  -> Lemma (requires (
     lbytes_eq salt1 salt2 /\ lbytes_eq ikm1 ikm2
   ))
   (ensures lbytes_eq (extract_prk3e2m salt1 ikm1) (extract_prk3e2m salt2 ikm2))
-  = ()
 
 val extract_prk4e3m:
   #cs:supported_cipherSuite
